More fixes

new/golang/defn/globals.v
@@ -5,12 +5,16 @@ Module globals.
 Section defns.
 Context `{ffi_syntax}.
 
+Definition unwrap : val :=
+  λ: "x", match: "x" with
+            NONE => #() #()
+          | SOME "x" => "x"
+          end.
+
 Definition get (pkg_var_name : (go_string * go_string)): val :=
   λ: <>,
-    match: GlobalGet #("vars:" ++ pkg_var_name.1) with
-      NONE => #() #()
-    | SOME "globalVarAddrs" => alist_lookup #(pkg_var_name.2) "globalVarAddrs"
-    end.
+    let: "varAddrs" := unwrap $ GlobalGet #("vars:" ++ pkg_var_name.1) in
+    unwrap $ alist_lookup #(pkg_var_name.2) "varAddrs".
 
 Fixpoint alloc (vars : list (go_string * go_type)) : val :=
   (λ: <>,
@@ -36,22 +40,17 @@ Context `{ffi_syntax}.
 
 Definition func_call (pkg_func_name : go_string * go_string) : val :=
   λ: <>,
-    match: GlobalGet #("funcs:" ++ pkg_func_name.1) with
-      NONE => #() #()
-    | SOME "funcs" => alist_lookup #(pkg_func_name.2) "funcs"
-    end.
+    let: "functions" := globals.unwrap $ GlobalGet #("funcs:" ++ pkg_func_name.1) in
+    globals.unwrap $ alist_lookup #(pkg_func_name.2) "functions".
 
 Definition method_call (pkg_type_method_name : go_string * go_string * go_string) : val :=
   λ: <>,
     let pkg_name := pkg_type_method_name.1.1 in
     let type_name := pkg_type_method_name.1.2 in
     let method_name := pkg_type_method_name.2 in
-    match: GlobalGet #("type:" ++ type_name) with
-      NONE => #() #()
-    | SOME "typeToMethodSet" =>
-        let: "methodSet" := (alist_lookup #type_name "globalVarAddrs") in
-        alist_lookup #method_name "methodSet"
-    end.
+    let: "typeToMethodSet" := globals.unwrap $ GlobalGet #("type:" ++ pkg_name) in
+    let: "methodSet" := globals.unwrap $ GlobalGet #("type:" ++ type_name) in
+    globals.unwrap $ alist_lookup #method_name "methodSet".
 
 End defns.
 
